Cslib/Computability/Machines/MultiTapeTuring/CopyRoutine.lean
@@ -13,6 +13,7 @@ public import Cslib.Computability.Machines.MultiTapeTuring.Basic
 public import Cslib.Computability.Machines.MultiTapeTuring.ListEncoding
 public import Cslib.Computability.Machines.MultiTapeTuring.HeadStats
 public import Cslib.Computability.Machines.MultiTapeTuring.WithTapes
+public import Cslib.Computability.Machines.MultiTapeTuring.TMWithAuxTapes
 
 -- TODO create a "common file"
 import Cslib.Computability.Machines.SingleTapeTuring.Basic
@@ -46,6 +47,25 @@ public lemma copy_eval_list
   {tapes : Fin k → List (List α)}
   (h_tapes_i : tapes ⟨i, h_i_lt⟩ ≠ []) :
   (copy i j (h_neq := h_neq) (h_i_lt) (h_j_lt)).eval_list tapes = Part.some
+    (Function.update tapes ⟨j, h_j_lt⟩
+      (((tapes ⟨i, h_i_lt⟩).head h_tapes_i) :: (tapes ⟨j, h_j_lt⟩))) := by
+  sorry
+
+public def copy' {k aux : ℕ} (i j : ℕ)
+  (h_neq : i ≠ j := by decide)
+  (h_i_lt : i < k := by decide)
+  (h_j_lt : j < k := by decide) :
+  MultiTapeTMWithAuxTapes k aux (WithSep α) :=
+  (copy₁.allocate_aux_tapes aux).with_tapes #v[⟨i, h_i_lt⟩, ⟨j, h_j_lt⟩]
+    (h_le_k := by omega)
+    (h_le_aux := by rfl)
+
+@[simp, grind =]
+public lemma copy'_eval_list
+  {k aux : ℕ} {i j : ℕ} {h_neq : i ≠ j} {h_i_lt : i < k} {h_j_lt : j < k}
+  {tapes : Fin k → List (List α)}
+  (h_tapes_i : tapes ⟨i, h_i_lt⟩ ≠ []) :
+  (copy' (aux := aux) i j (h_neq := h_neq) (h_i_lt) (h_j_lt)).eval_list tapes = Part.some
     (Function.update tapes ⟨j, h_j_lt⟩
       (((tapes ⟨i, h_i_lt⟩).head h_tapes_i) :: (tapes ⟨j, h_j_lt⟩))) := by
   sorry
