Cslib/Computability/Machines/MultiTapeTuring/SuccRoutine.lean
@@ -12,6 +12,8 @@ import Cslib.Foundations.Data.RelatesInSteps
 public import Cslib.Computability.Machines.MultiTapeTuring.Basic
 public import Cslib.Computability.Machines.MultiTapeTuring.ListEncoding
 public import Cslib.Computability.Machines.MultiTapeTuring.WithTapes
+public import Cslib.Computability.Machines.MultiTapeTuring.TMWithAuxTapes
+
 import Mathlib.Data.Nat.Bits
 
 namespace Turing
@@ -76,6 +78,23 @@ public theorem succ_eval_list {k : ℕ} {i : Fin k.succ} {tapes : Fin k.succ →
   (succ i).eval_list tapes = .some (succ_f i tapes) := by
   -- TOOD why does simp not find it?
   simp [MultiTapeTM.eval_of_computes succ_computes]
+
+public def succ' {k aux : ℕ} (i : ℕ) (h_i_lt : i < k := by decide) :
+    MultiTapeTMWithAuxTapes k aux (WithSep OneTwo) :=
+  (succ₀.allocate_aux_tapes aux).with_tapes #v[⟨i, h_i_lt⟩]
+    (h_le_k := by omega)
+    (h_le_aux := by rfl)
+
+@[simp, grind =]
+public lemma succ'_eval_list {k aux : ℕ} {i : ℕ} {h_i_lt : i < k}
+    {tapes : Fin k → List (List OneTwo)} :
+  (succ' (aux := aux) i h_i_lt).eval_list tapes = .some (
+    if h_ne : tapes ⟨i, h_i_lt⟩ ≠ [] then
+      Function.update tapes ⟨i, h_i_lt⟩
+        ((dya ((dya_inv ((tapes ⟨i, h_i_lt⟩).head h_ne)).succ)) :: (tapes ⟨i, h_i_lt⟩).tail)
+    else
+      tapes) := by
+  sorry
 
 public lemma succ₀_evalWithStats_list {n : ℕ} {ls : List (List OneTwo)} :
   succ₀.evalWithStats_list [(dya n) :: ls].get =
