Cslib/Computability/Machines/MultiTapeTuring/TMWithAuxTapes.lean
@@ -11,15 +11,7 @@ import Cslib.Foundations.Data.RelatesInSteps
 
 public import Cslib.Computability.Machines.MultiTapeTuring.Basic
 public import Cslib.Computability.Machines.MultiTapeTuring.ListEncoding
-public import Cslib.Computability.Machines.MultiTapeTuring.SuccRoutine
-public import Cslib.Computability.Machines.MultiTapeTuring.CopyRoutine
-public import Cslib.Computability.Machines.MultiTapeTuring.PushRoutine
-public import Cslib.Computability.Machines.MultiTapeTuring.PopRoutine
-public import Cslib.Computability.Machines.MultiTapeTuring.WhileCombinator
-public import Cslib.Computability.Machines.MultiTapeTuring.SequentialCombinator
 public import Cslib.Computability.Machines.MultiTapeTuring.WithTapes
-public import Cslib.Computability.Machines.MultiTapeTuring.IteCombinator
-public import Cslib.Computability.Machines.MultiTapeTuring.EqualRoutine
 
 namespace Turing
 
